% https://mindinloop.com/course/12
Let \((S′,R′)\) be a transition system with \(S′=\{s_0,s_1\}\) and
\(R′=\{(s_0,s_1), (s_1, s_1)\}\). For the following transition
system, we have \(S = \{s_0,s_1, s_2\}\), \(R = \{(s_0,s_0),(s_0,s_1),(s_1,
s_0)\}\), and we have \(S′ \subseteq S\) but \(R′ \not \subseqeq R\)
since \((s_1,s_1)\) is missing from R.

For the following transition system, we have \(S = \{s_0, s_1, s_2\}, R =
\{(s_0, s_1), (s_1, s_1), (s_2, s_1)\}\), and we have \(S' \subseteq S\) and
\(R' \subseteq R\).

For the following transitions system, we have \(S = \{s_0, s_1\}, R = \{(s_0,
s_0), (s_0, s_1), (s_1, s_1)\}\), and we have \(S' \subseteq S\) and \(R'
\subseteq R\).
