\documentclass{article}

\usepackage[utf8]{inputenc}
\usepackage{graphicx}
\usepackage{caption}
\usepackage{float}
\usepackage{color}
\usepackage{epigraph}
\usepackage[hang,flushmargin]{footmisc} 
\usepackage{tikz}
\usepackage{hyperref}
\hypersetup{pdfauthor={Cristian Adrián Ontivero}}
\usetikzlibrary{automata, positioning, arrows,
fit, % for the dashed boxes on Thompson's construction
calc
}
\tikzset{%
  node distance=3cm, % specifies the minimum distance between two nodes. Change if necessary.
  every state/.style={thick}, % sets the properties for each ’state’ node
  double distance=2.5pt,
  shorten >= 2pt, shorten <= 2pt,
  initial text=$ $,
  every edge/.style={%
    draw,->, >=stealth, auto, semithick
  }
}
\graphicspath{{imgs/}}

\definecolor{darkblue}{RGB}{49,130,189}

\newlength\tindent
\setlength{\tindent}{\parindent}
\setlength{\parindent}{0pt}
\renewcommand{\indent}{\hspace*{\tindent}}

%These tell TeX which packages to use.
\usepackage{array,epsfig}
\usepackage{amsmath}
\usepackage{amsfonts}
\usepackage{amssymb}
\usepackage{amsxtra}
\usepackage{amsthm}
\usepackage{mathrsfs}
\usepackage{color}

%Here I define some theorem styles and shortcut commands for symbols I use often
\theoremstyle{definition}
\newtheorem{defn}{Definition}
\newtheorem{thm}{Teorema}
\newtheorem{cor}{Corolario}
\newtheorem*{rmk}{Remark}
\newtheorem{lem}{Lema}
\newtheorem*{joke}{Joke}

\newtheorem{ex}{Example}
\newcommand{\exautorefname}{Ejemplo}

\newtheorem{exercise}{Ejercicio}
\newcommand{\exerciseautorefname}{Ejercicio}

\newtheorem{soln}{Solución}
\newtheorem{prop}{Proposición}

\newcommand{\lra}{\longrightarrow}
\newcommand{\ra}{\rightarrow}
\newcommand{\surj}{\twoheadrightarrow}
\newcommand{\graph}{\mathrm{graph}}
\newcommand{\bb}[1]{\mathbb{#1}}
\newcommand{\Z}{\bb{Z}}
\newcommand{\Q}{\bb{Q}}
\newcommand{\R}{\bb{R}}
\newcommand{\C}{\bb{C}}
\newcommand{\N}{\bb{N}}
\newcommand{\M}{\mathbf{M}}
\newcommand{\m}{\mathbf{m}}
\newcommand{\MM}{\mathscr{M}}
\newcommand{\HH}{\mathscr{H}}
\newcommand{\Om}{\Omega}
\newcommand{\Ho}{\in\HH(\Om)}
\newcommand{\bd}{\partial}
\newcommand{\del}{\partial}
\newcommand{\bardel}{\overline\partial}
\newcommand{\textdf}[1]{\textbf{\textsf{#1}}\index{#1}}
\newcommand{\img}{\mathrm{img}}
\newcommand{\ip}[2]{\left\langle{#1},{#2}\right\rangle}
\newcommand{\inter}[1]{\mathrm{int}{#1}}
\newcommand{\exter}[1]{\mathrm{ext}{#1}}
\newcommand{\cl}[1]{\mathrm{cl}{#1}}
\newcommand{\ds}{\displaystyle}
\newcommand{\vol}{\mathrm{vol}}
\newcommand{\cnt}{\mathrm{ct}}
\newcommand{\osc}{\mathrm{osc}}
\newcommand{\LL}{\mathbf{L}}
\newcommand{\UU}{\mathbf{U}}
\newcommand{\support}{\mathrm{support}}
\newcommand{\AND}{\;\wedge\;}
\newcommand{\OR}{\;\vee\;}
\newcommand{\Oset}{\varnothing}
\newcommand{\st}{\ni}
\newcommand{\wh}{\widehat}

\newcommand{\PS}{\mathcal{P}}
\newcommand{\set}[1]{\left\{#1\right\}}
\newcommand{\bra}[1]{\left[#1\right]}
\newcommand{\abs}[1]{\left|#1\right|}
\newcommand{\emptystr}{\varepsilon}
\newcommand{\emptylan}{\emptyset}
\newcommand{\pdv}[2]{\partial_{#1} \bigl(#2\bigr)}

%Pagination stuff.
\setlength{\topmargin}{-.3 in}
\setlength{\oddsidemargin}{0in}
\setlength{\evensidemargin}{0in}
\setlength{\textheight}{9.in}
\setlength{\textwidth}{6.5in}
\pagestyle{empty}

% Print today's date in ISO format (YYYY-MM-DD).
\def\isodate{\leavevmode\hbox{\the\year-\twodigits\month-\twodigits\day}}
\def\twodigits#1{\ifnum#1<10 0\fi\the#1}

% The problem environment is a regular ams theorem environment with "Problem"
% text and some leading space to give some separation between the problems.
\theoremstyle{definition}
\newtheorem{problem-internal}{Problem}[subsection]
\newenvironment{problem}{
  \medskip
  \begin{problem-internal}
}{
  \end{problem-internal}
}

% The solution environment is a proof environment with the "solution" text as
% well as the following adjustments:
% - No indent on paragraphs;
% - A small amount of space between paragraphs.
%
% Note: The negative space at the beginning is to remove the space before the
% first paragraph in the solution.
\newenvironment{solution}{%
  \begin{proof}[Solution]
  \vspace{-8px}
  \setlength{\parskip}{4px}
  \setlength{\parindent}{0px}
}{
  \end{proof}
}

\begin{document}
\begin{center}
  {\LARGE Algebra: Chapter 0}\\[.2cm]
  Cristian Adrián Ontivero \\[.05cm]%
\end{center}

\begin{solution}
Suppose $\sim$ is an equivalence relation on a set $S$.
Since $\sim$ is reflexive, $\forall x \in S (x \sim x) $, so $\forall x\in S
(x \in {[x]}_{\sim})$. Thus, no equivalence class is empty, and their union is
the whole set $S$.  It remains to show the disjointness of the equivalence
classes.  Let $x$ and $y$ be two elements of $S$. Suppose ${[x]}_{\sim} \cap
{[y]}_{\sim} \neq \emptyset$. Then there exists $z \in {[x]}_{\sim} \cap
{[y]}_{\sim}$, i.e. $z \in {[x]}_{\sim} \wedge z \in {[y]}_{\sim}$. By
definition of equivalence class, $z \sim x$ and $z \sim y$. By symmetry $x \sim
z$, and by transitivity $x \sim y$. Once more, by symmetry $y \sim x$. Knowing
all this, we proceed to prove that ${[x]}_{\sim} = {[y]}_{\sim}$.
\begin{itemize}
\item[$\subseteq$:] Let $d \in {[x]}_{\sim}$, this means that $d \sim x$. By
transitivity $d \sim y$, so $d \in {[y]}_{\sim}$.
\item[$\supseteq$:] Let $d \in {[y]}_{\sim}$, this means that $d \sim y$. By
transitivity $d \in x$, so $d \in {[x]}_{\sim}$.
\end{itemize}

Thus ${[x]}_{\sim} = {[y]}_{\sim}$.
\end{solution}

\begin{solution}
1.3 Given a partition $\mathcal{P}$ on a set $S$, we define a relation $\sim$ on
$S$ as follows: $x \sim y$ iff $x, y \in X$, for some $X \in \mathcal{P}$.
Let's prove that $\sim$ is an equivalence relation on S.
\begin{itemize}
  \item Reflexive: Let $x \in S$ be arbitrary. $x \in X$ for some $X \in
    \mathcal{P}$, so $x \sim x$.
  \item Symmetric: Let $x, y \in S$ be such that $x \sim y$ and $y \sim z$.
Then by definition of $\sim$ there ixists an $X \in \PS$ such that $x, y \in X$.
This also means that $x, y \in X$, thus $y \sim x$.
  \item Transitive: Let $x, y, z \in S$ be such that $x \sim y$ and $y \sim z$.
Then by definition $x, y \in X_1$ and $y,z \in X_2$, with $X_1, X_2 \in \PS$.
Since $\PS$ is a partition, $y$ is only in one part, thus $X_1 = X_2$. Therefore
$x, z \in X_1$, so $x \sim z$.
\end{itemize}
It now remains to prove that $\PS$ is $\PS_{\sim}$, the set of equivalence classes of $\sim$. Let $X \in \PS$ be a part of the partition. By definition of $\sim$, $\forall x, y \in X (x \sim y)$. Furthermore, given $a \in X$ and $S - X$ we know by definition that $a$ and $b$ are not related. Thus $X$ is an equivalence class of $\sim$. Finally, since every element of $S$ is in exactly one of the parts of $\PS$, we have that there are no equivalence classes besides the ones from the partition. Therefore $\PS$ is the set of equivalence classes of $\sim$.
\end{solution}

\begin{solution}
1.4 Five. These are:
\begin{align*}
  \sim_1 &= \set{(1,1), (2,2), (3,3)} \\
  \sim_2 &= \set{(1,1), (1,2), (2,1), (2,2), (3,3)} \\
  \sim_3 &= \set{(1,1), (1,3), (3,1), (3,3), (2,2)} \\
  \sim_4 &= \set{(1,1), (2,2), (2,3), (3,2), (3,3)} \\
  \sim_5 &= \set{(1,1), (1,2), (1,3), (2,2), (2,1), (2,3), (3,1), (3,2), (3,3)}
\end{align*}
This might be easier to think in terms of how many partitions of $\set{1,2,3}$ we can make:
\begin{align*}
  \PS_1 &= \set{\{1\}, \{2\}, \{3\}} \\
  \PS_2 &= \set{\{1, 2\}, \{3\}} \\
  \PS_3 &= \set{\{1, 3\}, \{2\}} \\
  \PS_4 &= \set{\{1\}, \{2, 3\}} \\
  \PS_5 &= \set{\{1, 2, 3\}}
\end{align*}
In general, the number of ways to partition a set of $n$ elements is given by the $n^{\text{th}}$ Bell number.
\end{solution}

\begin{solution}
1.5 Take $S = \set{1,2,3}$ and $R = \set{(1,1), (2,2), (3,3), (1,2), (2,1),
(2,3), (3,2)}$. $R$ is reflexive and symmetric, but not transitive. Recall that
an equivalence class of $x$ with respect to $R$ is
\[ \bra{x}_R = \set{y \in S \mid yRx} \]
Thus we have $\bra{1}_R = \set{1,2}$ and $\bra{2}_R = \set{1,2,3}$. Clearly
$\bra{1}_R \neq \bra{2}_R$, but they aren't disjoint ($\bra{1}_R \cap \bra{2}_R
\neq \emptyset$), so they can't form a partition.
\end{solution}

\begin{solution}
1.6 $\forall a, b \in \R (a \sim b \iff b - a \in \Z)$.
\begin{itemize}
\item Reflexive: $\forall a \in R, a \sim a \iff a - a = 0 \in Z$
\item Symmetric: Let $a,b \in \R$ by such that $a \sim b$. Then $b - a \in Z$, so its opposite $-(b-a) \in Z$, i.e. $a-b \in Z$, thus $b \sim a$.
\item Transitive: Let $a, b, c \in \R$ by such that $a \sim b$ and $b \sim c$. Then $b - a \in Z$, and $c - b \in Z$. Since $\Z$ is closed under addition, $(b-a) + (c-b) = c - a \in Z$. Thus $a \sim c$.
\end{itemize}
Under $\sim$ all reals with the same decimal expansion belong to the same
equivalence class. In other words $\forall x \in [0,1), \bra{x}_{\sim} = \set{n + x \mid n \in \Z}$.
In particular $\bra{0} = \Z$. Thus $\R/\sim = \R/\Z$ which is isomorphic to
$[0,1)$ and the unit circle (the book until here doesn't get into quotient
groups though!).

\[ \forall (a_1, a_2), (b_1, b_2) \in \R \times \R, (a_1, a_2) \approx (b_1, b_2) \iff b_1 - a_1, b_2 - a_2 \in Z \]

\begin{itemize}
\item Reflexive: Let $(a_1, a_2) \in \R^2$, $(a_1, a_2) \approx (a_1, a_2) \iff a_1 - a_1 = 0 \in \Z$ and $a_2 - a_2 = 0 \in \Z$.
\item Symmetric: Let $(a_1, a_2), (b_1, b_2) \in \R^2$ be such that $(a_1, a_2) \approx (b_1, b_2)$.
Then $b_1 - a_1 \in \Z \AND -(b_2 - a_1) \in \Z$, i.e.  $a_1 -b_1 \in \Z \AND a_2 - b_2 \in \Z$.
Therefore $(b_1, b_2) \approx (a_1, a_2)$.
\item Transitive: Let $(a_1, a_2), (b_1, b_2), (c_1, c_2) \in \R^2$ be such that $(a_1, a_2) \approx (b_1, b_2)$ and $(b_1, b_2) \approx (c_1, c_2)$. Then $(b_1 - a_1), (b_2 - a_2), (c_1 - b_1), (c_2 - b_2) \in \Z$, so $(b_1 - a_1) + (c_1 - b_1) = c_1 - a_1 \in \Z$ and $(b_2 - a_2) + (c_2 - b_2) = c_2 - a_2 \in \Z$, because $\Z$ is closed under addition. Therefore $(a_1, a_2) \approx (c_1, c_2)$.
\end{itemize}
\end{solution}

Check from section 2.5
Let $f \colon A \to B$ be a bijection, and define $g \colon B \to A$ by $g(b) = a$ whenever $f(a) = b$. We need to show that $g$, the flip of $\Gamma_f$ is a function according to the definition given, that is: 
\[ (\forall b \in B)(\exists! a \in A) (b,a) \in \Gamma_g \]
We prove it by contradiction. Suppose $\neg (\forall b \in B)(\exists! a \in A) (b,a) \in \Gamma_g$. This is equivalent to $\exists b \in B \neg (\exists! a \in A) (b,a) \in \Gamma_g$. Take this $b$. Either there is no element in $A$ such that $(b,a) \in \Gamma_g$, or there is more than one.
\begin{itemize}
\item Suppose $\neg \exists a \in A$ such that $(b,a) \in \Gamma_g$: then
$g(b)$ isn't defined, which by the way $g$ is defined implies that $f$ isn't
surjective, which is absurd.
\item Suppose there is more than one: then there are at least two different ones. Call them $c$ and $d$. Then $g(b) = c \AND g(b) = d \AND c \neq d$. By how $g$ is defined, this implies that $f(c) = b$, $f(d) = b$, and $c \neq d$, meaning that $f$ isn't injective, which is absurd.
\end{itemize}
Thus $(\forall b \in B)(\exists! a \in A) (b,a) \in \Gamma_g$.

Corollary 2.2: See Proposition 4.2

Canonical decomposition (2.8) (p.15)
\begin{itemize}
\item Reflexive: Let $a \in A$, $f(a) = f(a)$, so $a \sim a$.
\item Symmetric: Let $a, b \in A$ be such that $a \sim b$. Then $f(a) = f(b)$. Since $=$ is symmetric, $f(b) = f(a)$, so $b \sim a$.
\item Transitive: Let $a, b, c \in A$ be such that $a \sim b$ and $b \sim c$. Then $f(a) = f(b)$ and $f(b) = f(c)$. Since $=$ is transitive, $f(a) = f(c)$, so $a \sim c$.
\end{itemize}

\begin{solution}
There are $n!$ different bijections from a set of $n$ elements to itself, which
amount to the different possible permutations of the set. Take the first
element. You can map it to any of the n elements. Once that has been chosen,
map a second element to the remaining $(n-1)$, and so on.
\end{solution}

\begin{solution}
2.2 Assume $A \neq \emptyset$ and let $f \colon A \to B$ be a function. To be proved: $f$ has a right-inverse iff it is surjective.
\begin{itemize}
\item[$\Longrightarrow$:] Suppose $f$ has a right-inverse, then there exists $g \colon B \to A$ such that $f \circ g = id_B$. We need to show that $f$ is surjective. Let $b \in B$. Then $\exists a \in A$, namely $g(b)$, such that $f(a) = b$. Hence $f$ is surjective.
\item[$\Longleftarrow$:] Suppose $f$ is surjective. For each $b \in B$ construct a set
\[ \Lambda_b = \set{(a,b) \mid a \in A, f(a) = b} \]
Every $\Lambda_b$ is nonempty due to $f$ begin surjective, so we can choose a
pair from each $\Lambda_b$ to define $g \colon B \to A$ by $g(b) = a$, where
$(a,b) \in \Lambda_b$. Since $b = f(a) = f(g(b)) = (f \circ g)(b)$, $g$ is a
right-inverse of $f$.
\end{itemize}
\end{solution}

\begin{solution}
2.3 Suppose $f$ is a bijection, and $f^{-1}$ its inverse. Then $f^{-1}$ is a bijection too, since it has $f$ as its inverse: 
\[f \circ f^{-1} = id_B \AND f^{-1} \circ f = id_A \]
where $f \colon A \to B$ and $f^{-1} \colon B \to A$.
\end{solution}
Let $f\colon A \to B$ and $g\colon B \to C$ be two bijections, with $f^{-1}$
and $g^{-1}$ their inverses, respectively. Then $g \circ f \colon A \to C$ is
also a bijection, with its inverse $(g\circ f)^{-1}\colon C \to A$ being $f^{-1} \circ g^{-1}$. To see this:

\[(g \circ f)\circ {(g\circ f)}^{-1} = (g\circ f) \circ (f^{-1}\circ g^{-1}) = g \circ id_B \circ g^{-1} = id_C \]
\[{(g\circ f)}^{-1}\circ (g \circ f) = (f^{-1}\circ g^{-1}) \circ (g\circ f) = f^{-1} \circ id_B \circ f = id_A \]

\begin{solution}
2.4 Let $A,B,C$ be sets. We need to show that the relation ``is isomorphic
to'', denoted $\cong$, is an equivalence relation.
\begin{itemize}
\item Reflexive: $id_A\colon A \to A$ is an isomorphism, so $A\cong A$.
\item Symmetric: Suppose $A \cong B$. Then there exists an isomorphism $f\colon A \to B$, and it has another isomorphism $f^{-1}\colon B \to A$ as its inverse. Thus $B\cong A$.
\item Transitive: Suppose $A\cong B$ and $B\cong C$. There there exists $f\colon A \to B$ and $g\colon B \to C$, both isomorphisms. From the previous problem we know that $(g \circ f)\colon A \to C$ is an isomorphism, so $A \cong C$.
\end{itemize}
\end{solution}

\begin{solution}
2.5 A function $f\colon A \to B$ is an epimorphism (or epi) if the following holds:
for all sets $Z$ and all functions $\alpha', \alpha''\colon B \to Z (\alpha' \circ f = \alpha'' \circ f) \implies \alpha' = \alpha'')$.

Proposition: a function is surjective iff it is an epimorphism.
Proof
\begin{itemize}
\item[$(\implies)$:] Suppose $f\colon A \to B$ is surjective. By proposition 2.1 there is a function $g\colon B \to A$ which is its right-inverse. Assume $\alpha',\alpha''$ are arbitrary functions from $B$ to another set $Z$, and that $\alpha' \circ f = \alpha'' \circ f$.
Composing on the right by $g$, and using the associtivity of composition:
\begin{align*}
(\alpha' \circ f)\circ g &= (\alpha''\circ f)\circ g \\
\alpha' \circ (f\circ g) &= \alpha''\circ (f\circ g) \\
\alpha' \circ (id_B) &= \alpha''\circ (id_B) \\
\alpha' &= \alpha''
\end{align*}
Thus $f$ is an epimorphism.
\item[$(\Longleftarrow)$:] We prove by contradiction. Suppose $f$ is not
surjective. Then there is some $b \in B$ such that $\forall a \in A (f(a) \neq
b)$.Take two functions $\alpha', \alpha''\colon B \to Z$ where $Z =
\set{z_1,z_2,\dots}$ has at least two elements. $\alpha'(b) = z_1$,
$\alpha''(b) = z_2$, and they agree on the rest of the points (say $\forall b' \in B - \set{b}, \alpha'(b') = \alpha''(b') = z_1)$.
Suppose $\alpha \circ f = \alpha'' \circ f$. Since $\alpha' \neq \alpha''$, $f$
cannot be epic. Therefore $f$ is surjective.
\end{itemize}
\end{solution}

\begin{solution}
2.6 Let $A, B$ be sets. Given a function $f\colon A\to B$, we can define a function $s\colon A \to A \times B$ as $s(a) = (a, f(a))$. Then:
\[ todo \]
i.e. $(\pi_A \circ g)(a) = \pi_A(g(a)) = \pi_A(a, f(a)) = a$.
\end{solution}

\end{document}


